generational/spec/GC.Gen.CheneyGraphReadiness.fsti
@@ -1829,6 +1829,11 @@ val chunked_cheney_gc_correct_after_preflight_full_policy_and_post_reachable_ima
         CReach.chunked_roots_valid_nonblue
           (CRem.chunked_minor_collection_roots minor major base_roots)
           r.capacity_major_out /\
+        (SpecMajorAlloc.major_fl_head_wosize major fp <
+         PromotionDemand.minor_promotion_demand minor + 1 ==>
+         CReach.chunked_roots_disjoint_from_chunk
+           (CRem.chunked_minor_collection_roots minor major base_roots)
+           fresh) /\
         chunked_major_chunks_above_zero_addr r.capacity_major_out /\
         chunked_major_objects_are_pointer_fields r.capacity_major_out /\
         CReach.chunked_major_field_zero_no_minor
